veric/juicy_view.v
@@ -1,0 +1,819 @@
+From iris.algebra Require Export gmap agree.
+From iris.algebra Require Import local_updates proofmode_classes big_op.
+From VST.zlist Require Import sublist.
+From VST.msl Require Import shares.
+From VST.veric Require Export base Memory share_alg dfrac view.
+From iris_ora.algebra Require Export ora gmap agree.
+From iris.prelude Require Import options.
+
+(* We can't import compcert.lib.Maps because their lookup notations conflict with stdpp's.
+   We can define lookup instances, which require one more ! apiece than CompCert's notation. *)
+Global Instance ptree_lookup A : Lookup positive A (Maps.PTree.t A) := Maps.PTree.get(A := A).
+Global Instance pmap_lookup A : LookupTotal positive A (Maps.PMap.t A) := Maps.PMap.get(A := A).
+
+Lemma perm_order''_refl : forall s, Mem.perm_order'' s s.
+Proof.
+  destruct s; simpl; try done.
+  apply perm_refl.
+Qed.
+
+Lemma perm_order''_trans: forall a b c, Mem.perm_order'' a b ->  Mem.perm_order'' b c ->
+                             Mem.perm_order'' a c.
+Proof.
+   intros a b c H1 H2; destruct a, b, c; inversion H1; inversion H2; subst; eauto;
+           eapply perm_order_trans; eauto.
+Qed.
+
+Lemma perm_order''_None : forall a, Mem.perm_order'' a None.
+Proof. destruct a; simpl; auto. Qed.
+
+Definition perm_of_sh (sh: Share.t): option permission :=
+  if writable0_share_dec sh
+  then if eq_dec sh Share.top
+          then Some Freeable
+          else Some Writable
+  else if readable_share_dec sh
+       then Some Readable
+       else if eq_dec sh Share.bot
+                 then None
+            else Some Nonempty.
+Functional Scheme perm_of_sh_ind := Induction for perm_of_sh Sort Prop.
+
+Definition perm_of_dfrac dq :=
+  match dq with
+  | DfracOwn sh => perm_of_sh sh
+  | DfracDiscarded => Some Readable
+  | DfracBoth sh => if Mem.perm_order'_dec (perm_of_sh sh) Readable then perm_of_sh sh else Some Readable
+  end.
+
+Definition perm_of_res' {V} (r: option (dfrac * V)) :=
+  match r with
+  | Some (dq, _) => perm_of_dfrac dq
+  | None => None
+  end.
+
+Lemma perm_of_sh_mono : forall (sh1 sh2 : shareR), sh1 ⋅ sh2 ≠ Share.bot -> Mem.perm_order'' (perm_of_sh (sh1 ⋅ sh2)) (perm_of_sh sh1).
+Proof.
+  intros ?? H.
+  pose proof (proj1 (share_op_equiv sh1 sh2 _) eq_refl) as J.
+  rewrite -> if_false in J by auto; destruct J as (? & ? & J).
+  unfold perm_of_sh.
+  destruct (writable0_share_dec sh1).
+  { eapply join_writable01 in w; eauto.
+    rewrite -> if_true by auto.
+    if_tac; if_tac; simpl; try constructor.
+    subst; rewrite -> (@only_bot_joins_top sh2) in H1 by (eexists; eauto); contradiction. }
+  if_tac; [repeat if_tac; constructor|].
+  destruct (readable_share_dec sh1).
+  { eapply join_readable1 in r; eauto.
+    rewrite (if_true _ _ _ _ _ r); constructor. }
+  repeat if_tac; try constructor; contradiction.
+Qed.
+
+Lemma perm_order_antisym : forall p1 p2, ~perm_order p1 p2 -> perm_order p2 p1.
+Proof.
+  destruct p1, p2; try constructor; intros X; contradiction X; constructor.
+Qed.
+
+Lemma perm_order'_antisym : forall p1 p2, ~Mem.perm_order' p1 p2 -> Mem.perm_order'' (Some p2) p1.
+Proof.
+  destruct p1; simpl; auto; apply perm_order_antisym.
+Qed.
+
+Lemma perm_of_dfrac_mono : forall d1 d2, ✓d2 -> d1 ≼ d2 -> Mem.perm_order'' (perm_of_dfrac d2) (perm_of_dfrac d1).
+Proof.
+  intros ?? Hv [d0 ->%leibniz_equiv].
+  destruct d1, d0; simpl in *; repeat if_tac; auto; try (apply perm_order''_refl || (by apply perm_of_sh_mono) || (by destruct Hv; apply perm_of_sh_mono) || constructor).
+  - by apply perm_order'_antisym.
+  - destruct Hv; eapply perm_order''_trans, perm_of_sh_mono; [apply perm_order'_antisym|]; eauto.
+  - destruct Hv; eapply perm_order''_trans, perm_of_sh_mono; [apply perm_order'_antisym|]; eauto.
+  - destruct Hv; eapply perm_order''_trans, perm_of_sh_mono; [apply perm_order'_antisym|]; eauto.
+Qed.
+
+Class resource_ops (V : ofe) := {
+  perm_of_res : option (dfrac * V) -> option permission;
+  memval_of : dfrac * V -> option memval;
+  perm_of_res_None : perm_of_res None = None;
+  perm_of_res_mono : forall d1 d2 (r : V), ✓d2 -> d1 ≼ d2 -> Mem.perm_order'' (perm_of_res (Some (d2, r))) (perm_of_res (Some (d1, r)));
+  perm_of_res_ne : forall n d (r1 r2 : V), r1 ≡{n}≡ r2 -> perm_of_res (Some (d, r1)) = perm_of_res (Some (d, r2));
+  perm_of_res_max : forall r, Mem.perm_order'' (perm_of_res' r) (perm_of_res r);
+  memval_of_mono : forall d1 d2 (r : V) v, memval_of (d1, r) = Some v -> d1 ≼ d2 -> memval_of (d2, r) = Some v;
+  memval_of_ne : forall n d (r1 r2 : V) v, memval_of (d, r1) = Some v -> r1 ≡{n}≡ r2 -> memval_of (d, r2) = Some v
+}.
+
+(** * ORA for a juicy mem. An algebra where a resource map is a view of a CompCert memory if it is
+      coherent with that memory. *)
+
+Local Definition juicy_view_fragUR (V : ofe) : uora :=
+  gmapUR address (prodR dfracR (agreeR V)).
+
+(** View relation. *)
+Section rel.
+  Context (V : ofe) {ResOps : resource_ops V}.
+  Implicit Types (m : Memory.mem) (k : address) (r : option (dfrac * V)) (v : memval) (n : nat).
+  Implicit Types (f : gmap address (dfrac * agree V)).
+
+  Notation rmap := (gmap address (dfrac * agree V)).
+
+  Definition elem_of_agree {A} (x : agree A) : { a | a ∈ agree_car x}.
+  Proof. destruct x as [[|a ?] ?]; [done | exists a; apply elem_of_cons; auto]. Qed.
+
+  Lemma elem_of_agree_ne : forall {A} n (x y : agreeR A), ✓{n} x -> x ≡{n}≡ y -> proj1_sig (elem_of_agree x) ≡{n}≡ proj1_sig (elem_of_agree y).
+  Proof.
+    intros; destruct (elem_of_agree x), (elem_of_agree y); simpl.
+    destruct (proj1 H0 _ e) as (? & Hv2 & ->).
+    rewrite H0 in H; eapply agree_validN_def; done.
+  Qed.
+
+  Definition resR_to_resource : optionR (prodR dfracR (agreeR V)) -> option (dfrac * V) :=
+    option_map (fun '(q, a) => (q, proj1_sig (elem_of_agree a))).
+
+  Definition resource_at f k := resR_to_resource (f !! k).
+  Local Infix "@" := resource_at (at level 50, no associativity).
+
+  Definition contents_at (m: mem) (loc: address) : memval :=
+    Maps.ZMap.get (snd loc) (Maps.PMap.get (fst loc) (Mem.mem_contents m)).
+
+  Definition contents_cohere (m: mem) k r :=
+    forall v, r ≫= memval_of = Some v -> contents_at m k = v.
+
+  Definition access_cohere (m: mem) k r :=
+    Mem.perm_order'' (access_at m k Cur) (perm_of_res r).
+
+  Definition max_access_at m loc := access_at m loc Max.
+
+  Definition max_access_cohere (m: mem) k r :=
+    Mem.perm_order'' (max_access_at m k) (perm_of_res' r).
+
+  Definition alloc_cohere (m: mem) k r :=
+    (fst k >= Mem.nextblock m)%positive -> r = None.
+
+  Definition coherent n (m : leibnizO mem) phi := ✓{n} phi ∧ forall loc, let r := phi @ loc in
+    contents_cohere m loc r ∧ access_cohere m loc r ∧ max_access_cohere m loc r ∧ alloc_cohere m loc r.
+
+  Local Lemma coherent_mono n1 n2 (m1 m2 : leibnizO mem) f1 f2 :
+    coherent n1 m1 f1 →
+    m1 ≡{n2}≡ m2 →
+    f2 ≼{n2} f1 →
+    n2 ≤ n1 →
+    coherent n2 m2 f2.
+  Proof using Type*.
+    intros (Hv & H) -> Hf Hn.
+    assert (✓{n2} f2) as Hv2.
+    { eapply cmra_validN_includedN; eauto.
+      eapply cmra_validN_le; eauto. }
+    split; first done.
+    intros loc; specialize (Hv loc); specialize (Hv2 loc); specialize (H loc).
+    rewrite lookup_includedN in Hf; specialize (Hf loc); rewrite option_includedN in Hf.
+    destruct H as (Hcontents & Hcur & Hmax & Halloc); unfold resource_at in *; repeat split.
+    - unfold contents_cohere in *; intros.
+      apply Hcontents.
+      destruct Hf as [Hf | ((d2, v2) & (d1, v1) & Hf2 & Hf1 & Hf)]; [rewrite Hf in H; inv H|].
+      rewrite Hf2 in H Hv2; inv H.
+      rewrite Hf1 /= in Hv |- *.
+      rewrite pair_includedN in Hf.
+      destruct Hv as [_ Hv], Hv2 as [_ Hv2].
+      eapply cmra_validN_le in Hv; eauto.
+      assert (v2 ≡{n2}≡ v1) as Hvs by (by destruct Hf as [[_ ?] | [_ ?%agree_valid_includedN]]).
+      rewrite H1; eapply memval_of_ne, elem_of_agree_ne, Hvs; auto.
+      destruct Hf as [[Hd _] | [Hd _]]; [by rewrite -discrete_iff /= in Hd; apply leibniz_equiv in Hd; subst|].
+      eapply memval_of_mono; eauto.
+    - unfold access_cohere in *.
+      destruct Hf as [Hf | ((?, v2) & (?, v1) & Hf2 & Hf1 & Hf)]; [rewrite Hf perm_of_res_None; apply perm_order''_None|].
+      eapply perm_order''_trans; [apply Hcur|].
+      rewrite Hf1 Hf2 /= in Hv Hv2 |- *.
+      rewrite pair_includedN in Hf.
+      destruct Hv as [? Hv], Hv2 as [_ Hv2].
+      eapply cmra_validN_le in Hv; eauto.
+      assert (v2 ≡{n2}≡ v1) as Hvs by (by destruct Hf as [[_ ?] | [_ ?%agree_valid_includedN]]).
+      erewrite <- perm_of_res_ne by (apply elem_of_agree_ne, Hvs; auto).
+      destruct Hf as [[Hd _] | [Hd _]]; [by rewrite -discrete_iff /= in Hd; apply leibniz_equiv in Hd; subst; apply perm_order''_refl|].
+      apply perm_of_res_mono; auto.
+    - unfold max_access_cohere in *.
+      destruct Hf as [Hf | ((?, v2) & (?, v1) & Hf2 & Hf1 & Hf)]; [rewrite Hf; apply perm_order''_None|].
+      eapply perm_order''_trans; [apply Hmax|].
+      rewrite Hf1 Hf2 /= in Hv Hv2 |- *.
+      rewrite pair_includedN in Hf.
+      destruct Hf as [[Hd _] | [Hd _]]; [by rewrite -discrete_iff /= in Hd; apply leibniz_equiv in Hd; subst; apply perm_order''_refl|].
+      destruct Hv; apply perm_of_dfrac_mono; auto.
+    - unfold alloc_cohere in *; intros H; specialize (Halloc H).
+      destruct Hf as [Hf | (? & ? & Hf2 & Hf1 & _)]; [by rewrite Hf|].
+      rewrite Hf1 in Halloc; discriminate.
+  Qed.
+
+  Local Lemma coherent_valid n m f :
+    coherent n m f → ✓{n} f.
+  Proof.
+    intros H; apply H.
+  Qed.
+
+  Local Lemma coherent_unit n :
+    ∃ m, coherent n m ε.
+  Proof using Type*.
+    exists Mem.empty; repeat split.
+    - intros ?; unfold resource_at.
+      rewrite lookup_empty; discriminate.
+    - unfold access_cohere, resource_at.
+      rewrite lookup_empty perm_of_res_None; apply perm_order''_None.
+  Qed.
+
+  Local Canonical Structure coherent_rel : view_rel (leibnizO mem) (juicy_view_fragUR V) :=
+    ViewRel coherent coherent_mono coherent_valid coherent_unit.
+
+  Definition access_of_rmap f b ofs (k : perm_kind) :=
+    match k with
+    | Max => perm_of_res' (f @ (b, ofs))
+    | Cur => perm_of_res (f @ (b, ofs))
+    end.
+
+  Definition make_access (next : Values.block) (r : rmap) :=
+    fold_right (fun b p => Maps.PTree.set b (access_of_rmap r b) p) (Maps.PTree.empty _)
+    (map Z.to_pos (tl (upto (Pos.to_nat next)))).
+
+  Lemma make_access_get_aux : forall l f b t,
+    Maps.PTree.get b (fold_right (fun b p => Maps.PTree.set b (access_of_rmap f b) p) t l) =
+    if In_dec eq_block b l then Some (access_of_rmap f b) else Maps.PTree.get b t.
+  Proof.
+    induction l; simpl; auto; intros.
+    destruct (eq_block a b).
+    - subst; apply Maps.PTree.gss.
+    - rewrite Maps.PTree.gso; last auto.
+      rewrite IHl.
+      if_tac; auto.
+  Qed.
+
+  Lemma make_access_get : forall next f b,
+    Maps.PTree.get b (make_access next f) =
+    if Pos.ltb b next then Some (access_of_rmap f b) else None.
+  Proof.
+    intros; unfold make_access.
+    rewrite make_access_get_aux.
+    if_tac; destruct (Pos.ltb_spec0 b next); auto.
+    - rewrite in_map_iff in H; destruct H as (? & ? & Hin); subst.
+      destruct (Pos.to_nat next) eqn: Hnext.
+      { pose proof (Pos2Nat.is_pos next); lia. }
+      simpl in Hin.
+      rewrite in_map_iff in Hin; destruct Hin as (? & ? & Hin); subst.
+      apply In_upto in Hin.
+      destruct x0; simpl in *; lia.
+    - contradiction H.
+      rewrite in_map_iff; do 2 eexists.
+      { apply Pos2Z.id. }
+      destruct (Pos.to_nat next) eqn: Hnext.
+      { pose proof (Pos2Nat.is_pos next); lia. }
+      simpl.
+      rewrite in_map_iff; do 2 eexists.
+      { rewrite -> Zminus_succ_l.
+        unfold Z.succ. rewrite -> Z.add_simpl_r; reflexivity. }
+      rewrite In_upto; lia.
+  Qed.
+
+  Definition make_contents (r : rmap) : Maps.PMap.t (Maps.ZMap.t memval) :=
+    map_fold (fun '(b, ofs) '(d, v) c => Maps.PMap.set b (Maps.ZMap.set ofs
+      (match memval_of (d, proj1_sig (elem_of_agree v)) with Some v => v | None => Undef end) (c !!! b)) c)
+      (Maps.PMap.init (Maps.ZMap.init Undef)) r.
+
+  Lemma make_contents_get : forall f (b : Values.block) ofs,
+    Maps.ZMap.get ofs ((make_contents f) !!! b) = match f @ (b, ofs) ≫= memval_of with Some v => v | _ => Undef end.
+  Proof.
+    intros; unfold make_contents.
+    apply (map_fold_ind (fun c f => Maps.ZMap.get ofs (c !!! b) = match f @ (b, ofs) ≫= memval_of with Some v => v | _ => Undef end)).
+    - rewrite /lookup_total /pmap_lookup Maps.PMap.gi Maps.ZMap.gi /resource_at lookup_empty //.
+    - intros (b1, ofs1) (d, v) ?? Hi H.
+      destruct (eq_dec b1 b).
+      + subst; rewrite /lookup_total /pmap_lookup Maps.PMap.gss.
+        destruct (eq_dec ofs1 ofs).
+        * subst; rewrite Maps.ZMap.gss /resource_at lookup_insert //.
+        * rewrite Maps.ZMap.gso; last done.
+          rewrite /resource_at lookup_insert_ne //.
+          congruence.
+      + rewrite /lookup_total /pmap_lookup Maps.PMap.gso; last done.
+        rewrite /resource_at lookup_insert_ne //.
+        congruence.
+  Qed.
+
+  Lemma make_contents_default : forall f (b : Values.block), (make_contents f !!! b).1 = Undef.
+  Proof.
+    intros; unfold make_contents.
+    apply (map_fold_ind (fun c f => (c !!! b).1 = Undef)); try done.
+    intros (b1, ofs) (?, ?) ????.
+    destruct (eq_dec b1 b).
+    - subst; rewrite /lookup_total /pmap_lookup Maps.PMap.gss //.
+    - rewrite /lookup_total /pmap_lookup Maps.PMap.gso //.
+  Qed.
+
+  Definition maxblock_of_rmap f := map_fold (fun '(b, _) _ c => Pos.max b c) 1%positive f.
+
+  Lemma maxblock_max : forall f b ofs, (b > maxblock_of_rmap f)%positive -> f !! (b, ofs) = None.
+  Proof.
+    intros ???; unfold maxblock_of_rmap.
+    apply (map_fold_ind (fun c f => (b > c)%positive -> f !! (b, ofs) = None)).
+    - by rewrite lookup_empty.
+    - intros (b1, ?) (?, ?) ??? IH ?.
+      destruct (eq_dec b1 b); first lia.
+      rewrite lookup_insert_ne; last congruence.
+      apply IH; lia.
+  Qed.
+
+  Program Definition mem_of_rmap f : mem :=
+    {| Mem.mem_contents := make_contents f;
+       Mem.mem_access := (fun _ _ => None, make_access (maxblock_of_rmap f + 1)%positive f);
+       Mem.nextblock := (maxblock_of_rmap f + 1)%positive |}.
+  Next Obligation.
+  Proof.
+    intros; rewrite /Maps.PMap.get make_access_get.
+    simple_if_tac; last done.
+    apply perm_of_res_max.
+  Qed.
+  Next Obligation.
+  Proof.
+    intros.
+    rewrite /Maps.PMap.get make_access_get.
+    destruct (Pos.ltb_spec b (maxblock_of_rmap f + 1)%positive); done.
+  Qed.
+  Next Obligation.
+  Proof.
+    apply make_contents_default.
+  Qed.
+
+  Lemma mem_of_rmap_coherent : forall n f, ✓{n} f -> coherent n (mem_of_rmap f) f.
+  Proof.
+    intros; split; first done.
+    intros (b, ofs); simpl.
+    repeat split.
+    - rewrite /contents_cohere /contents_at /= => ? Hv.
+      rewrite make_contents_get Hv //.
+    - rewrite /access_cohere /access_at /=.
+      rewrite /Maps.PMap.get make_access_get.
+      destruct (Pos.ltb_spec b (maxblock_of_rmap f + 1)%positive).
+      + apply perm_order''_refl.
+      + simpl. rewrite /resource_at maxblock_max; last lia.
+        rewrite perm_of_res_None //.
+    - rewrite /max_access_cohere /max_access_at /access_at /=.
+      rewrite /Maps.PMap.get make_access_get.
+      destruct (Pos.ltb_spec b (maxblock_of_rmap f + 1)%positive).
+      + apply perm_order''_refl.
+      + simpl. rewrite /resource_at maxblock_max //; lia.
+    - rewrite /alloc_cohere /= => ?.
+      rewrite /resource_at maxblock_max //; lia.
+  Qed.
+
+  Local Lemma coherent_rel_exists n f :
+    (∃ m, coherent_rel n m f) ↔ ✓{n} f.
+  Proof.
+    split.
+    - intros [m Hrel]. eapply coherent_valid, Hrel.
+    - intros; eexists; apply mem_of_rmap_coherent; auto.
+  Qed.
+
+  Local Lemma coherent_rel_unit n m : coherent_rel n m ε.
+  Proof.
+    split. { apply uora_unit_validN. }
+    simpl; intros; rewrite /resource_at lookup_empty /=.
+    repeat split; try done.
+    - rewrite /access_cohere perm_of_res_None; apply perm_order''_None.
+    - rewrite /max_access_cohere; apply perm_order''_None.
+  Qed.
+
+  Local Lemma coherent_rel_discrete :
+    OfeDiscrete V → ViewRelDiscrete coherent_rel.
+  Proof.
+    intros ? n m f [Hv Hrel].
+    split; last done.
+    by apply cmra_discrete_valid_iff_0.
+  Qed.
+
+  Lemma rmap_orderN_includedN : ∀n f1 f2, ✓{n} f2 -> f1 ≼ₒ{n} f2 -> f1 ≼{n} f2.
+  Proof.
+    intros ??? Hv; rewrite lookup_includedN; intros.
+    specialize (H i); specialize (Hv i).
+    destruct (f1 !! i) as [(d1, v1)|] eqn: Hf1, (f2 !! i) as [(d2, v2)|] eqn: Hf2; rewrite ?Hf1 Hf2 /= in H Hv |- *; try done.
+    - rewrite Some_includedN pair_includedN; destruct Hv, H as [Hd Hv]; simpl in *.
+      apply agree_order_dist in Hv as ->; last done.
+      destruct Hd; subst; auto.
+      right; split; auto; eexists; eauto.
+    - rewrite option_includedN; auto.
+  Qed.
+
+  Local Lemma coherent_rel_order : ∀n a x y, x ≼ₒ{n} y → coherent_rel n a y → coherent_rel n a x.
+  Proof.
+    intros ???? Hord [? Hy].
+    eapply coherent_mono; first (by split); auto.
+    apply rmap_orderN_includedN; auto.
+  Qed.
+
+End rel.
+
+Local Existing Instance coherent_rel_discrete.
+
+(** [juicy_view] is a notation to give canonical structure search the chance
+to infer the right instances (see [auth]). *)
+Notation juicy_view V := (view (@coherent _ _ V)).
+Definition juicy_viewO (V : ofe) `{resource_ops V} : ofe := viewO (coherent_rel V).
+Definition juicy_viewC (V : ofe) `{resource_ops V} : cmra := viewC (coherent_rel V).
+Definition juicy_viewUC (V : ofe) `{resource_ops V} : ucmra := viewUC (coherent_rel V).
+Canonical Structure juicy_viewR (V : ofe) `{resource_ops V} : ora := view.viewR (coherent_rel V) (coherent_rel_order V).
+Canonical Structure juicy_viewUR (V : ofe) `{resource_ops V} : uora := viewUR (coherent_rel V).
+
+Section definitions.
+  Context {V : ofe} {ResOps : resource_ops V}.
+
+  Definition juicy_view_auth (dq : dfrac) (m : leibnizO mem) : juicy_viewUR V :=
+    ●V{dq} m.
+  Definition juicy_view_frag (k : address) (dq : dfrac) (v : V) : juicy_viewUR V :=
+    ◯V {[k := (dq, to_agree v)]}.
+End definitions.
+
+Section lemmas.
+  Context {V : ofe} {ResOps : resource_ops V}.
+  Implicit Types (m : mem) (q : shareR) (dq : dfrac) (v : V).
+
+  Global Instance : Params (@juicy_view_auth) 3 := {}.
+  Global Instance juicy_view_auth_ne dq : NonExpansive (juicy_view_auth (V:=V) dq).
+  Proof. solve_proper. Qed.
+  Global Instance juicy_view_auth_proper dq : Proper ((≡) ==> (≡)) (juicy_view_auth (V:=V) dq).
+  Proof. apply ne_proper, _. Qed.
+
+  Global Instance : Params (@juicy_view_frag) 4 := {}.
+  Global Instance juicy_view_frag_ne k oq : NonExpansive (juicy_view_frag (V:=V) k oq).
+  Proof. solve_proper. Qed.
+  Global Instance juicy_view_frag_proper k oq : Proper ((≡) ==> (≡)) (juicy_view_frag (V:=V) k oq).
+  Proof. apply ne_proper, _. Qed.
+
+  (* Helper lemmas *)
+(*  Local Lemma coherent_rel_lookup n m k dq v :
+    coherent_rel V n m {[k := (dq, to_agree v)]} ↔ ✓ dq ∧ m !! k ≡{n}≡ Some v.
+  Proof.
+    split.
+    - intros Hrel.
+      edestruct (Hrel k) as (v' & Hagree & Hval & ->).
+      { rewrite lookup_singleton. done. }
+      simpl in *. apply (inj _) in Hagree. rewrite Hagree.
+      done.
+    - intros [Hval (v' & Hm & Hv')%dist_Some_inv_r'] j [df va].
+      destruct (decide (k = j)) as [<-|Hne]; last by rewrite lookup_singleton_ne.
+      rewrite lookup_singleton. intros [= <- <-]. simpl.
+      exists v'. split_and!; by rewrite ?Hv'.
+  Qed. *)
+
+  (** Composition and validity *)
+  Lemma juicy_view_auth_dfrac_op dp dq m :
+    juicy_view_auth (dp ⋅ dq) m ≡
+    juicy_view_auth dp m ⋅ juicy_view_auth dq m.
+  Proof. by rewrite /juicy_view_auth view_auth_dfrac_op. Qed.
+  Global Instance juicy_view_auth_dfrac_is_op dq dq1 dq2 m :
+    IsOp dq dq1 dq2 → IsOp' (juicy_view_auth dq m) (juicy_view_auth dq1 m) (juicy_view_auth dq2 m).
+  Proof. rewrite /juicy_view_auth. apply _. Qed.
+
+  Lemma juicy_view_auth_dfrac_op_invN n dp m1 dq m2 :
+    ✓{n} (juicy_view_auth dp m1 ⋅ juicy_view_auth dq m2) → m1 = m2.
+  Proof. by intros ?%view_auth_dfrac_op_invN. Qed.
+  Lemma juicy_view_auth_dfrac_op_inv dp m1 dq m2 :
+    ✓ (juicy_view_auth dp m1 ⋅ juicy_view_auth dq m2) → m1 = m2.
+  Proof. by intros ?%view_auth_dfrac_op_inv. Qed.
+
+  Lemma juicy_view_auth_dfrac_validN m n dq : ✓{n} juicy_view_auth dq m ↔ ✓ dq.
+  Proof.
+    rewrite view_auth_dfrac_validN. intuition. apply coherent_rel_unit.
+  Qed.
+  Lemma juicy_view_auth_dfrac_valid m dq : ✓ juicy_view_auth dq m ↔ ✓ dq.
+  Proof.
+    rewrite view_auth_dfrac_valid. intuition. apply coherent_rel_unit.
+  Qed.
+  Lemma juicy_view_auth_valid m : ✓ juicy_view_auth (DfracOwn Tsh) m.
+  Proof. rewrite juicy_view_auth_dfrac_valid. done. Qed.
+
+  Lemma juicy_view_auth_dfrac_op_validN n dq1 dq2 m1 m2 :
+    ✓{n} (juicy_view_auth dq1 m1 ⋅ juicy_view_auth dq2 m2) ↔ ✓ (dq1 ⋅ dq2) ∧ m1 = m2.
+  Proof.
+    rewrite view_auth_dfrac_op_validN. intuition. apply coherent_rel_unit.
+  Qed.
+  Lemma juicy_view_auth_dfrac_op_valid dq1 dq2 m1 m2 :
+    ✓ (juicy_view_auth dq1 m1 ⋅ juicy_view_auth dq2 m2) ↔ ✓ (dq1 ⋅ dq2) ∧ m1 = m2.
+  Proof.
+    rewrite view_auth_dfrac_op_valid. intuition. apply coherent_rel_unit.
+  Qed.
+
+  Lemma juicy_view_auth_op_validN n m1 m2 :
+    ✓{n} (juicy_view_auth (DfracOwn Tsh) m1 ⋅ juicy_view_auth (DfracOwn Tsh) m2) ↔ False.
+  Proof. apply view_auth_op_validN. Qed.
+  Lemma juicy_view_auth_op_valid m1 m2 :
+    ✓ (juicy_view_auth (DfracOwn Tsh) m1 ⋅ juicy_view_auth (DfracOwn Tsh) m2) ↔ False.
+  Proof. apply view_auth_op_valid. Qed.
+
+  Lemma juicy_view_frag_validN n k dq v : ✓{n} juicy_view_frag k dq v ↔ ✓ dq.
+  Proof.
+    rewrite view_frag_validN coherent_rel_exists singleton_validN pair_validN.
+    naive_solver.
+  Qed.
+  Lemma juicy_view_frag_valid k dq v : ✓ juicy_view_frag k dq v ↔ ✓ dq.
+  Proof.
+    rewrite cmra_valid_validN. setoid_rewrite juicy_view_frag_validN.
+    naive_solver eauto using O.
+  Qed.
+
+  Lemma juicy_view_frag_op k dq1 dq2 v :
+    juicy_view_frag k (dq1 ⋅ dq2) v ≡ juicy_view_frag k dq1 v ⋅ juicy_view_frag k dq2 v.
+  Proof. rewrite -view_frag_op singleton_op -cmra.pair_op agree_idemp //. Qed.
+  Lemma juicy_view_frag_add k q1 q2 v :
+    juicy_view_frag k (DfracOwn (q1 ⋅ q2)) v ≡
+      juicy_view_frag k (DfracOwn q1) v ⋅ juicy_view_frag k (DfracOwn q2) v.
+  Proof. rewrite -juicy_view_frag_op. done. Qed.
+
+  Lemma juicy_view_frag_op_validN n k dq1 dq2 v1 v2 :
+    ✓{n} (juicy_view_frag k dq1 v1 ⋅ juicy_view_frag k dq2 v2) ↔
+      ✓ (dq1 ⋅ dq2) ∧ v1 ≡{n}≡ v2.
+  Proof.
+    rewrite view_frag_validN coherent_rel_exists singleton_op singleton_validN.
+    by rewrite -cmra.pair_op pair_validN to_agree_op_validN.
+  Qed.
+  Lemma juicy_view_frag_op_valid k dq1 dq2 v1 v2 :
+    ✓ (juicy_view_frag k dq1 v1 ⋅ juicy_view_frag k dq2 v2) ↔ ✓ (dq1 ⋅ dq2) ∧ v1 ≡ v2.
+  Proof.
+    rewrite view_frag_valid. setoid_rewrite coherent_rel_exists.
+    rewrite -cmra_valid_validN singleton_op singleton_valid.
+    by rewrite -cmra.pair_op pair_valid to_agree_op_valid.
+  Qed.
+  (* FIXME: Having a [valid_L] lemma is not consistent with [auth] and [view]; they
+     have [inv_L] lemmas instead that just have an equality on the RHS. *)
+  Lemma juicy_view_frag_op_valid_L `{!LeibnizEquiv V} k dq1 dq2 v1 v2 :
+    ✓ (juicy_view_frag k dq1 v1 ⋅ juicy_view_frag k dq2 v2) ↔ ✓ (dq1 ⋅ dq2) ∧ v1 = v2.
+  Proof. unfold_leibniz. apply juicy_view_frag_op_valid. Qed.
+
+(*  Lemma juicy_view_both_dfrac_validN n dp m k dq v :
+    ✓{n} (juicy_view_auth dp m ⋅ juicy_view_frag k dq v) ↔
+      ✓ dp ∧ ✓ dq ∧ m !! k ≡{n}≡ Some v.
+  Proof.
+    rewrite /juicy_view_auth /juicy_view_frag.
+    rewrite view_both_dfrac_validN coherent_rel_lookup.
+    naive_solver.
+  Qed.
+  Lemma juicy_view_both_validN n m k dq v :
+    ✓{n} (juicy_view_auth (DfracOwn Tsh) m ⋅ juicy_view_frag k dq v) ↔
+      ✓ dq ∧ m !! k ≡{n}≡ Some v.
+  Proof. rewrite juicy_view_both_dfrac_validN. naive_solver done. Qed.
+  Lemma juicy_view_both_dfrac_valid dp m k dq v :
+    ✓ (juicy_view_auth dp m ⋅ juicy_view_frag k dq v) ↔
+    ✓ dp ∧ ✓ dq ∧ m !! k ≡ Some v.
+  Proof.
+    rewrite /juicy_view_auth /juicy_view_frag.
+    rewrite view_both_dfrac_valid. setoid_rewrite coherent_rel_lookup.
+    split=>[[Hq Hm]|[Hq Hm]].
+    - split; first done. split.
+      + apply (Hm 0%nat).
+      + apply equiv_dist=>n. apply Hm.
+    - split; first done. intros n. split.
+      + apply Hm.
+      + revert n. apply equiv_dist. apply Hm.
+  Qed.
+  Lemma juicy_view_both_dfrac_valid_L `{!LeibnizEquiv V} dp m k dq v :
+    ✓ (juicy_view_auth dp m ⋅ juicy_view_frag k dq v) ↔
+    ✓ dp ∧ ✓ dq ∧ m !! k = Some v.
+  Proof. unfold_leibniz. apply juicy_view_both_dfrac_valid. Qed.
+  Lemma juicy_view_both_valid m k dq v :
+    ✓ (juicy_view_auth (DfracOwn Tsh) m ⋅ juicy_view_frag k dq v) ↔
+    ✓ dq ∧ m !! k ≡ Some v.
+  Proof. rewrite juicy_view_both_dfrac_valid. naive_solver done. Qed.
+  (* FIXME: Having a [valid_L] lemma is not consistent with [auth] and [view]; they
+     have [inv_L] lemmas instead that just have an equality on the RHS. *)
+  Lemma juicy_view_both_valid_L `{!LeibnizEquiv V} m k dq v :
+    ✓ (juicy_view_auth (DfracOwn Tsh) m ⋅ juicy_view_frag k dq v) ↔
+    ✓ dq ∧ m !! k = Some v.
+  Proof. unfold_leibniz. apply juicy_view_both_valid. Qed.
+
+  (** Frame-preserving updates *)
+  Lemma juicy_view_alloc m k dq v :
+    m !! k = None →
+    ✓ dq →
+    juicy_view_auth (DfracOwn Tsh) m ~~> juicy_view_auth (DfracOwn Tsh) (<[k := v]> m) ⋅ juicy_view_frag k dq v.
+  Proof.
+    intros Hfresh Hdq. apply view_update_alloc=>n bf Hrel j [df va] /=.
+    rewrite lookup_op. destruct (decide (j = k)) as [->|Hne].
+    - assert (bf !! k = None) as Hbf.
+      { destruct (bf !! k) as [[df' va']|] eqn:Hbf; last done.
+        specialize (Hrel _ _ Hbf). destruct Hrel as (v' & _ & _ & Hm).
+        exfalso. rewrite Hm in Hfresh. done. }
+      rewrite lookup_singleton Hbf.
+      intros [= <- <-]. eexists. do 2 (split; first done).
+      rewrite lookup_insert. done.
+    - rewrite lookup_singleton_ne; last done.
+      rewrite left_id=>Hbf.
+      specialize (Hrel _ _ Hbf). destruct Hrel as (v' & ? & ? & Hm).
+      eexists. do 2 (split; first done).
+      rewrite lookup_insert_ne //.
+  Qed.
+
+  Lemma juicy_view_alloc_big m m' dq :
+    m' ##ₘ m →
+    ✓ dq →
+    juicy_view_auth (DfracOwn Tsh) m ~~>
+      juicy_view_auth (DfracOwn Tsh) (m' ∪ m) ⋅ ([^op map] k↦v ∈ m', juicy_view_frag k dq v).
+  Proof.
+    intros. induction m' as [|k v m' ? IH] using map_ind; decompose_map_disjoint.
+    { rewrite big_opM_empty left_id_L right_id. done. }
+    rewrite IH //.
+    rewrite big_opM_insert // assoc.
+    apply cmra_update_op; last done.
+    rewrite -insert_union_l. apply (juicy_view_alloc _ k dq); last done.
+    by apply lookup_union_None.
+  Qed.
+
+  Lemma juicy_view_delete m k v :
+    juicy_view_auth (DfracOwn Tsh) m ⋅ juicy_view_frag k (DfracOwn Tsh) v ~~>
+    juicy_view_auth (DfracOwn Tsh) (delete k m).
+  Proof.
+    apply view_update_dealloc=>n bf Hrel j [df va] Hbf /=.
+    destruct (decide (j = k)) as [->|Hne].
+    - edestruct (Hrel k) as (v' & _ & Hdf & _).
+      { rewrite lookup_op Hbf lookup_singleton -Some_op. done. }
+      exfalso. apply: dfrac_full_exclusive. apply Hdf.
+    - edestruct (Hrel j) as (v' & ? & ? & Hm).
+      { rewrite lookup_op lookup_singleton_ne // Hbf. done. }
+      exists v'. do 2 (split; first done).
+      rewrite lookup_delete_ne //.
+  Qed.
+
+  Lemma juicy_view_delete_big m m' :
+    juicy_view_auth (DfracOwn Tsh) m ⋅ ([^op map] k↦v ∈ m', juicy_view_frag k (DfracOwn Tsh) v) ~~>
+    juicy_view_auth (DfracOwn Tsh) (m ∖ m').
+  Proof.
+    induction m' as [|k v m' ? IH] using map_ind.
+    { rewrite right_id_L big_opM_empty right_id //. }
+    rewrite big_opM_insert //.
+    rewrite [juicy_view_frag _ _ _ ⋅ _]comm assoc IH juicy_view_delete.
+    rewrite -delete_difference. done.
+  Qed.
+
+  Lemma juicy_view_update m k v v' :
+    juicy_view_auth (DfracOwn Tsh) m ⋅ juicy_view_frag k (DfracOwn Tsh) v ~~>
+      juicy_view_auth (DfracOwn Tsh) (<[k := v']> m) ⋅ juicy_view_frag k (DfracOwn Tsh) v'.
+  Proof.
+    rewrite juicy_view_delete.
+    rewrite (juicy_view_alloc _ k (DfracOwn Tsh) v') //; last by rewrite lookup_delete.
+    rewrite insert_delete_insert //.
+  Qed.
+
+  Lemma juicy_view_update_big m m0 m1 :
+    dom m0 = dom m1 →
+    juicy_view_auth (DfracOwn Tsh) m ⋅ ([^op map] k↦v ∈ m0, juicy_view_frag k (DfracOwn Tsh) v) ~~>
+      juicy_view_auth (DfracOwn Tsh) (m1 ∪ m) ⋅ ([^op map] k↦v ∈ m1, juicy_view_frag k (DfracOwn Tsh) v).
+  Proof.
+    intros Hdom%eq_sym. revert m1 Hdom.
+    induction m0 as [|k v m0 Hnotdom IH] using map_ind; intros m1 Hdom.
+    { rewrite dom_empty_L in Hdom.
+      apply dom_empty_iff_L in Hdom as ->.
+      rewrite left_id_L big_opM_empty. done. }
+    rewrite dom_insert_L in Hdom.
+    assert (k ∈ dom m1) as Hindom by set_solver.
+    apply elem_of_dom in Hindom as [v' Hlookup].
+    rewrite big_opM_insert //.
+    rewrite [juicy_view_frag _ _ _ ⋅ _]comm assoc.
+    rewrite (IH (delete k m1)); last first.
+    { rewrite dom_delete_L Hdom.
+      apply not_elem_of_dom in Hnotdom. set_solver -Hdom. }
+    rewrite -assoc [_ ⋅ juicy_view_frag _ _ _]comm assoc.
+    rewrite (juicy_view_update _ _ _ v').
+    rewrite (big_opM_delete _ m1 k v') // -assoc.
+    rewrite insert_union_r; last by rewrite lookup_delete.
+    rewrite union_delete_insert //.
+  Qed.*)
+
+  Lemma juicy_view_auth_persist dq m :
+    juicy_view_auth dq m ~~> juicy_view_auth DfracDiscarded m.
+  Proof. apply view_update_auth_persist. Qed.
+
+(*  Lemma juicy_view_frag_persist k dq v :
+    juicy_view_frag k dq v ~~> juicy_view_frag k DfracDiscarded v.
+  Proof.
+    apply view_update_frag=>m n bf Hrel.
+    eapply coherent_mono; first apply Hrel; auto.
+    apply (@cmra_monoN_r (juicy_view_fragUR V)).
+    rewrite singleton_includedN_l lookup_singleton.
+    eexists; split; first done.
+    rewrite Some_includedN pair_includedN; right.
+    split; last by apply to_agree_includedN.
+    eexists.
+Search DfracDiscarded includedN.
+    hnf.
+    Search to_agree includedN.
+    rewrite lookup_singleton.
+Search includedN "singleton".
+    rewrite lookup_includedN.
+    Search op includedN.
+    rewrite lookup_op. destruct (decide (j = k)) as [->|Hne].
+    - rewrite lookup_singleton.
+      edestruct (Hrel k ((dq, to_agree v) ⋅? bf !! k)) as (v' & Hdf & Hva & Hm).
+      { rewrite lookup_op lookup_singleton.
+        destruct (bf !! k) eqn:Hbf; by rewrite Hbf. }
+      rewrite Some_op_opM. intros [= Hbf].
+      exists v'. rewrite assoc; split; last done.
+      destruct (bf !! k) as [[df' va']|] eqn:Hbfk; rewrite Hbfk in Hbf; clear Hbfk.
+      + simpl in *. rewrite -cmra.pair_op in Hbf.
+        move:Hbf=>[= <- <-]. split; first done.
+        eapply cmra_discrete_valid.
+        eapply (dfrac_discard_update _ _ (Some df')).
+        apply cmra_discrete_valid_iff. done.
+      + simpl in *. move:Hbf=>[= <- <-]. split; done.
+    - rewrite lookup_singleton_ne //.
+      rewrite left_id=>Hbf.
+      edestruct (Hrel j) as (v'' & ? & ? & Hm).
+      { rewrite lookup_op lookup_singleton_ne // left_id. done. }
+      simpl in *. eexists. do 2 (split; first done). done.
+  Qed.*)
+
+  (** Typeclass instances *)
+  Global Instance juicy_view_frag_core_id k dq v : OraCoreId dq → OraCoreId (juicy_view_frag k dq v).
+  Proof. apply _. Qed.
+
+  Global Instance juicy_view_ora_discrete : OfeDiscrete V → OraDiscrete (juicy_viewR V).
+  Proof. apply _. Qed.
+
+  Global Instance juicy_view_frag_mut_is_op dq dq1 dq2 k v :
+    IsOp dq dq1 dq2 →
+    IsOp' (juicy_view_frag k dq v) (juicy_view_frag k dq1 v) (juicy_view_frag k dq2 v).
+  Proof. rewrite /IsOp' /IsOp => ->. apply juicy_view_frag_op. Qed.
+End lemmas.
+
+(*
+(** Functor *)
+Program Definition juicy_viewURF (F : oFunctor) : uorarFunctor := {|
+  uorarFunctor_car A _ B _ := juicy_viewUR (oFunctor_car F A B);
+  uorarFunctor_map A1 _ A2 _ B1 _ B2 _ fg :=
+    viewO_map (rel:=coherent_rel (oFunctor_car F A1 B1))
+              (rel':=coherent_rel (oFunctor_car F A2 B2))
+              (gmapO_map (oFunctor_map F fg))
+              (gmapO_map (prodO_map cid (agreeO_map (oFunctor_map F fg))))
+|}.
+Next Obligation.
+  intros K ?? F A1 ? A2 ? B1 ? B2 ? n f g Hfg.
+  apply viewO_map_ne.
+  - apply gmapO_map_ne, oFunctor_map_ne. done.
+  - apply gmapO_map_ne. apply prodO_map_ne; first done.
+    apply agreeO_map_ne, oFunctor_map_ne. done.
+Qed.
+Next Obligation.
+  intros K ?? F A ? B ? x; simpl in *. rewrite -{2}(view_map_id x).
+  apply (view_map_ext _ _ _ _)=> y.
+  - rewrite /= -{2}(map_fmap_id y).
+    apply map_fmap_equiv_ext=>k ??.
+    apply oFunctor_map_id.
+  - rewrite /= -{2}(map_fmap_id y).
+    apply map_fmap_equiv_ext=>k [df va] ?.
+    split; first done. simpl.
+    rewrite -{2}(agree_map_id va).
+    eapply agree_map_ext; first by apply _.
+    apply oFunctor_map_id.
+Qed.
+Next Obligation.
+  intros K ?? F A1 ? A2 ? A3 ? B1 ? B2 ? B3 ? f g f' g' x; simpl in *.
+  rewrite -view_map_compose.
+  apply (view_map_ext _ _ _ _)=> y.
+  - rewrite /= -map_fmap_compose.
+    apply map_fmap_equiv_ext=>k ??.
+    apply oFunctor_map_compose.
+  - rewrite /= -map_fmap_compose.
+    apply map_fmap_equiv_ext=>k [df va] ?.
+    split; first done. simpl.
+    rewrite -agree_map_compose.
+    eapply agree_map_ext; first by apply _.
+    apply oFunctor_map_compose.
+Qed.
+Next Obligation.
+  intros K ?? F A1 ? A2 ? B1 ? B2 ? fg; simpl.
+  (* [apply] does not work, probably the usual unification probem (Coq #6294) *)
+  apply: view_map_ora_morphism; [apply _..|]=> n m f.
+  intros Hrel k [df va] Hf. move: Hf.
+  rewrite !lookup_fmap.
+  destruct (f !! k) as [[df' va']|] eqn:Hfk; rewrite Hfk; last done.
+  simpl=>[= <- <-].
+  specialize (Hrel _ _ Hfk). simpl in Hrel. destruct Hrel as (v & Hagree & Hdval & Hm).
+  exists (oFunctor_map F fg v).
+  rewrite Hm. split; last by auto.
+  rewrite Hagree. rewrite agree_map_to_agree. done.
+Qed.
+
+Global Instance juicy_viewURF_contractive (K : Type) `{Countable K} F :
+  oFunctorContractive F → uorarFunctorContractive (juicy_viewURF K F).
+Proof.
+  intros ? A1 ? A2 ? B1 ? B2 ? n f g Hfg.
+  apply viewO_map_ne.
+  - apply gmapO_map_ne. apply oFunctor_map_contractive. done.
+  - apply gmapO_map_ne. apply prodO_map_ne; first done.
+    apply agreeO_map_ne, oFunctor_map_contractive. done.
+Qed.
+
+Program Definition juicy_viewRF (K : Type) `{Countable K} (F : oFunctor) : OrarFunctor := {|
+  orarFunctor_car A _ B _ := juicy_viewR K (oFunctor_car F A B);
+  orarFunctor_map A1 _ A2 _ B1 _ B2 _ fg :=
+    viewO_map (rel:=coherent_rel K (oFunctor_car F A1 B1))
+              (rel':=coherent_rel K (oFunctor_car F A2 B2))
+              (gmapO_map (K:=K) (oFunctor_map F fg))
+              (gmapO_map (K:=K) (prodO_map cid (agreeO_map (oFunctor_map F fg))))
+|}.
+Solve Obligations with apply juicy_viewURF.
+
+Global Instance juicy_viewRF_contractive (K : Type) `{Countable K} F :
+  oFunctorContractive F → OrarFunctorContractive (juicy_viewRF K F).
+Proof. apply juicy_viewURF_contractive. Qed.*)
+
+Global Typeclasses Opaque juicy_view_auth juicy_view_frag.
