veric/resource_map.v
@@ -1,0 +1,318 @@
+(* modified from iris.base_logic.lib.resource_map *)
+
+(** A "ghost map" (or "ghost heap") with a proposition controlling authoritative
+ownership of the entire heap, and a "points-to-like" proposition for (mutable,
+fractional, or persistent read-only) ownership of individual elements. *)
+From iris.proofmode Require Import proofmode.
+From iris_ora.logic Require Export logic own.
+From VST.veric Require Export shares share_alg.
+From VST.veric Require Import view juicy_view ext_order.
+From iris.prelude Require Import options.
+Export Address.
+
+Class resource_mapG Σ (V : Type) `{resource_ops (leibnizO V)} := GhostMapG {
+  resource_map_inG : inG Σ (juicy_viewR (leibnizO V));
+}.
+Local Existing Instance resource_map_inG.
+
+Definition resource_mapΣ (V : Type) `{resource_ops (leibnizO V)} : gFunctors :=
+  #[ GFunctor (juicy_viewR (leibnizO V)) ].
+
+Global Instance subG_resource_mapΣ Σ (V : Type) `{resource_ops (leibnizO V)} :
+  subG (resource_mapΣ V) Σ → resource_mapG Σ V.
+Proof. solve_inG. Qed.
+
+Section definitions.
+  Context `{resource_mapG Σ V} `{resource_ops (leibnizO V)}.
+
+  Local Definition resource_map_auth_def
+      (γ : gname) (q : share) (m : mem) : iProp Σ :=
+    own γ (juicy_view_auth (V:=leibnizO V) (DfracOwn q) m).
+  Local Definition resource_map_auth_aux : seal (@resource_map_auth_def).
+  Proof. by eexists. Qed.
+  Definition resource_map_auth := resource_map_auth_aux.(unseal).
+  Local Definition resource_map_auth_unseal :
+    @resource_map_auth = @resource_map_auth_def := resource_map_auth_aux.(seal_eq).
+
+  Local Definition resource_map_elem_def
+      (γ : gname) (k : address) (dq : dfrac) (v : V) : iProp Σ :=
+    own γ (juicy_view_frag (V:=leibnizO V) k dq v).
+  Local Definition resource_map_elem_aux : seal (@resource_map_elem_def).
+  Proof. by eexists. Qed.
+  Definition resource_map_elem := resource_map_elem_aux.(unseal).
+  Local Definition resource_map_elem_unseal :
+    @resource_map_elem = @resource_map_elem_def := resource_map_elem_aux.(seal_eq).
+End definitions.
+
+Notation "k ↪[ γ ] dq v" := (resource_map_elem γ k dq v)
+  (at level 20, γ at level 50, dq custom dfrac at level 1,
+   format "k  ↪[ γ ] dq  v") : bi_scope.
+
+Local Ltac unseal := rewrite
+  ?resource_map_auth_unseal /resource_map_auth_def
+  ?resource_map_elem_unseal /resource_map_elem_def.
+
+Section lemmas.
+  Context `{resource_mapG Σ V} `{resource_ops (leibnizO V)}.
+  Implicit Types (k : address) (v : V) (dq : dfrac) (q : shareR).
+
+  (** * Lemmas about the map elements *)
+  Global Instance resource_map_elem_timeless k γ dq v : Timeless (k ↪[γ]{dq} v).
+  Proof. unseal. apply _. Qed.
+  Global Instance resource_map_elem_persistent k γ v : Persistent (k ↪[γ]□ v).
+  Proof. unseal. apply _. Qed.
+(*  Global Instance resource_map_elem_fractional k γ v : Fractional (λ q, k ↪[γ]{#q} v)%I.
+  Proof. unseal. intros p q. rewrite -own_op juicy_view_frag_add //. Qed.
+  Global Instance resource_map_elem_as_fractional k γ q v :
+    AsFractional (k ↪[γ]{#q} v) (λ q, k ↪[γ]{#q} v)%I q.
+  Proof. split; first done. apply _. Qed.*)
+  Global Instance resource_map_elem_affine k γ v : Affine (k ↪[γ]□ v).
+  Proof. unseal. apply _. Qed.
+
+  Local Lemma resource_map_elems_unseal γ m dq :
+    ([∗ map] k ↦ v ∈ m, k ↪[γ]{dq} v) ==∗
+    own γ ([^op map] k↦v ∈ m, juicy_view_frag (V:=leibnizO V) k dq v).
+  Proof.
+    unseal. destruct (decide (m = ∅)) as [->|Hne].
+    - rewrite !big_opM_empty. iIntros "_". iApply own_unit.
+    - rewrite big_opM_own //. iIntros "?". done.
+  Qed.
+
+  Lemma resource_map_elem_valid k γ dq v : k ↪[γ]{dq} v -∗ ⌜✓ dq⌝.
+  Proof.
+    unseal. iIntros "Helem".
+    iDestruct (own_valid with "Helem") as %?%juicy_view_frag_valid.
+    done.
+  Qed.
+  Lemma resource_map_elem_valid_2 k γ dq1 dq2 v1 v2 :
+    k ↪[γ]{dq1} v1 -∗ k ↪[γ]{dq2} v2 -∗ ⌜✓ (dq1 ⋅ dq2) ∧ v1 = v2⌝.
+  Proof.
+    unseal. iIntros "H1 H2".
+    iDestruct (own_valid_2 with "H1 H2") as %?%juicy_view_frag_op_valid.
+    done.
+  Qed.
+  Lemma resource_map_elem_agree k γ dq1 dq2 v1 v2 :
+    k ↪[γ]{dq1} v1 -∗ k ↪[γ]{dq2} v2 -∗ ⌜v1 = v2⌝.
+  Proof.
+    iIntros "Helem1 Helem2".
+    iDestruct (resource_map_elem_valid_2 with "Helem1 Helem2") as %[_ ?].
+    done.
+  Qed.
+
+  Global Instance resource_map_elem_combine_gives γ k v1 dq1 v2 dq2 : 
+    CombineSepGives (k ↪[γ]{dq1} v1) (k ↪[γ]{dq2} v2) ⌜✓ (dq1 ⋅ dq2) ∧ v1 = v2⌝.
+  Proof.
+    rewrite /CombineSepGives. iIntros "[H1 H2]".
+    iDestruct (resource_map_elem_valid_2 with "H1 H2") as %[??].
+    eauto.
+  Qed.
+
+  Lemma resource_map_elem_combine k γ dq1 dq2 v1 v2 :
+    k ↪[γ]{dq1} v1 -∗ k ↪[γ]{dq2} v2 -∗ k ↪[γ]{dq1 ⋅ dq2} v1 ∧ ⌜v1 = v2⌝.
+  Proof.
+    iIntros "Hl1 Hl2". iDestruct (resource_map_elem_agree with "Hl1 Hl2") as %->.
+    unseal. iCombine "Hl1 Hl2" as "Hl". rewrite -own_op juicy_view_frag_op. eauto with iFrame.
+  Qed.
+
+  Global Instance resource_map_elem_combine_as k γ dq1 dq2 v1 v2 :
+    CombineSepAs (k ↪[γ]{dq1} v1) (k ↪[γ]{dq2} v2) (k ↪[γ]{dq1 ⋅ dq2} v1) | 60. 
+    (* higher cost than the Fractional instance [combine_sep_fractional_bwd],
+       which kicks in for #qs *)
+  Proof.
+    rewrite /CombineSepAs. iIntros "[H1 H2]".
+    iDestruct (resource_map_elem_combine with "H1 H2") as "[$ _]".
+  Qed.
+
+  Lemma resource_map_elem_split k γ dq1 dq2 v :
+    k ↪[γ]{dq1 ⋅ dq2} v ⊣⊢ k ↪[γ]{dq1} v ∗ k ↪[γ]{dq2} v.
+  Proof.
+    unseal. by rewrite -own_op juicy_view_frag_op.
+  Qed.
+
+  Lemma resource_map_elem_frac_ne γ k1 k2 dq1 dq2 v1 v2 :
+    ¬ ✓ (dq1 ⋅ dq2) → k1 ↪[γ]{dq1} v1 -∗ k2 ↪[γ]{dq2} v2 -∗ ⌜k1 ≠ k2⌝.
+  Proof.
+    iIntros (?) "H1 H2"; iIntros (->).
+    by iDestruct (resource_map_elem_valid_2 with "H1 H2") as %[??].
+  Qed.
+  Lemma resource_map_elem_ne γ k1 k2 dq2 v1 v2 :
+    k1 ↪[γ] v1 -∗ k2 ↪[γ]{dq2} v2 -∗ ⌜k1 ≠ k2⌝.
+  Proof. apply resource_map_elem_frac_ne. apply: exclusive_l. Qed.
+
+  (** Make an element read-only. *)
+(*  Lemma resource_map_elem_persist k γ dq v :
+    k ↪[γ]{dq} v ==∗ k ↪[γ]□ v.
+  Proof. unseal. iApply own_update. apply juicy_view_frag_persist. Qed. *)
+
+(*  (** * Lemmas about [resource_map_auth] *)
+  Lemma resource_map_alloc_strong P m :
+    pred_infinite P →
+    ⊢ |==> ∃ γ, ⌜P γ⌝ ∧ resource_map_auth γ Tsh m ∗ [∗ map] k ↦ v ∈ m, k ↪[γ] v.
+  Proof.
+    unseal. intros.
+    iMod (own_alloc_strong (juicy_view_auth (V:=leibnizO V) (DfracOwn Tsh) ∅) P)
+      as (γ) "[% Hauth]".
+    { apply juicy_view_auth_valid. }
+    iExists γ. iFrame "%".
+    rewrite -big_opM_own_1 -own_op. iApply (own_update with "Hauth").
+    etrans; first apply: (juicy_view_alloc_big (V:=leibnizO V) _ m (DfracOwn Tsh)).
+    - apply map_disjoint_empty_r.
+    - done.
+    - rewrite right_id. done.
+  Qed.
+  Lemma resource_map_alloc_strong_empty P :
+    pred_infinite P →
+    ⊢ |==> ∃ γ, ⌜P γ⌝ ∧ resource_map_auth γ Tsh (∅ : gmap K V).
+  Proof.
+    intros. iMod (resource_map_alloc_strong P ∅) as (γ) "(% & Hauth & _)"; eauto.
+  Qed.
+  Lemma resource_map_alloc m :
+    ⊢ |==> ∃ γ, resource_map_auth γ Tsh m ∗ [∗ map] k ↦ v ∈ m, k ↪[γ] v.
+  Proof.
+    iMod (resource_map_alloc_strong (λ _, True) m) as (γ) "[_ Hmap]".
+    - by apply pred_infinite_True.
+    - eauto.
+  Qed.
+  Lemma resource_map_alloc_empty :
+    ⊢ |==> ∃ γ, resource_map_auth γ Tsh (∅ : gmap K V).
+  Proof.
+    intros. iMod (resource_map_alloc ∅) as (γ) "(Hauth & _)"; eauto.
+  Qed.*)
+
+  Global Instance resource_map_auth_timeless γ q m : Timeless (resource_map_auth γ q m).
+  Proof. unseal. apply _. Qed.
+(*  Global Instance resource_map_auth_fractional γ m : Fractional (λ q, resource_map_auth γ q m)%I.
+  Proof. intros p q. unseal. rewrite -own_op -juicy_view_auth_dfrac_op //. Qed.
+  Global Instance resource_map_auth_as_fractional γ q m :
+    AsFractional (resource_map_auth γ q m) (λ q, resource_map_auth γ q m)%I q.
+  Proof. split; first done. apply _. Qed.*)
+
+  Lemma resource_map_auth_valid γ q m : resource_map_auth γ q m -∗ ⌜q ≠ Share.bot⌝.
+  Proof.
+    unseal. iIntros "Hauth".
+    iDestruct (own_valid with "Hauth") as %?%juicy_view_auth_dfrac_valid.
+    done.
+  Qed.
+  Lemma resource_map_auth_valid_2 γ q1 q2 m1 m2 :
+    resource_map_auth γ q1 m1 -∗ resource_map_auth γ q2 m2 -∗ ⌜q1 ⋅ q2 ≠ Share.bot ∧ m1 = m2⌝.
+  Proof.
+    unseal. iIntros "H1 H2".
+    iDestruct (own_valid_2 with "H1 H2") as %[??]%juicy_view_auth_dfrac_op_valid.
+    done.
+  Qed.
+  Lemma resource_map_auth_agree γ q1 q2 m1 m2 :
+    resource_map_auth γ q1 m1 -∗ resource_map_auth γ q2 m2 -∗ ⌜m1 = m2⌝.
+  Proof.
+    iIntros "H1 H2".
+    iDestruct (resource_map_auth_valid_2 with "H1 H2") as %[_ ?].
+    done.
+  Qed.
+
+  (** * Lemmas about the interaction of [resource_map_auth] with the elements *)
+(*  Lemma resource_map_lookup {γ q m k dq v} :
+    resource_map_auth γ q m -∗ k ↪[γ]{dq} v -∗ ⌜m !! k = Some v⌝.
+  Proof.
+    unseal. iIntros "Hauth Hel".
+    iDestruct (own_valid_2 with "Hauth Hel") as %[?[??]]%juicy_view_both_dfrac_valid_L.
+    eauto.
+  Qed.*)
+
+(*  Global Instance resource_map_lookup_combine_gives_1 {γ q m k dq v} :
+    CombineSepGives (resource_map_auth γ q m) (k ↪[γ]{dq} v) ⌜m !! k = Some v⌝.
+  Proof.
+    rewrite /CombineSepGives. iIntros "[H1 H2]".
+    iDestruct (resource_map_lookup with "H1 H2") as %->. eauto.
+  Qed.
+
+  Global Instance resource_map_lookup_combine_gives_2 {γ q m k dq v} :
+    CombineSepGives (k ↪[γ]{dq} v) (resource_map_auth γ q m) ⌜m !! k = Some v⌝.
+  Proof.
+    rewrite /CombineSepGives comm. apply resource_map_lookup_combine_gives_1.
+  Qed. *)
+
+(*  Lemma resource_map_insert {γ m} k v :
+    m !! k = None →
+    resource_map_auth γ Tsh m ==∗ resource_map_auth γ Tsh (<[k := v]> m) ∗ k ↪[γ] v.
+  Proof.
+    unseal. intros ?. rewrite -own_op.
+    iApply own_update. apply: juicy_view_alloc; done.
+  Qed.
+  Lemma resource_map_insert_persist {γ m} k v :
+    m !! k = None →
+    resource_map_auth γ Tsh m ==∗ resource_map_auth γ Tsh (<[k := v]> m) ∗ k ↪[γ]□ v.
+  Proof.
+    iIntros (?) "Hauth".
+    iMod (resource_map_insert k with "Hauth") as "[$ Helem]".
+    iApply resource_map_elem_persist. done.
+  Qed.
+
+  Lemma resource_map_delete {γ m k v} :
+    resource_map_auth γ Tsh m -∗ k ↪[γ] v ==∗ resource_map_auth γ Tsh (delete k m).
+  Proof.
+    unseal. apply bi.wand_intro_r. rewrite -own_op.
+    iApply own_update. apply: juicy_view_delete.
+  Qed.
+
+  Lemma resource_map_update {γ m k v} w :
+    resource_map_auth γ Tsh m -∗ k ↪[γ] v ==∗ resource_map_auth γ Tsh (<[k := w]> m) ∗ k ↪[γ] w.
+  Proof.
+    unseal. apply bi.wand_intro_r. rewrite -!own_op.
+    apply own_update. apply: juicy_view_update.
+  Qed.
+
+  (** Big-op versions of above lemmas *)
+  Lemma resource_map_lookup_big {γ q m} m0 :
+    resource_map_auth γ q m -∗
+    ([∗ map] k↦v ∈ m0, k ↪[γ] v) -∗
+    ⌜m0 ⊆ m⌝.
+  Proof.
+    iIntros "Hauth Hfrag". rewrite map_subseteq_spec. iIntros (k v Hm0).
+    rewrite big_sepM_lookup_acc; last done.
+    iDestruct "Hfrag" as "[Hfrag ?]".
+    iDestruct (resource_map_lookup with "Hauth Hfrag") as %->.
+    done.
+  Qed.
+
+  Lemma resource_map_insert_big {γ m} m' :
+    m' ##ₘ m →
+    resource_map_auth γ Tsh m ==∗
+    resource_map_auth γ Tsh (m' ∪ m) ∗ ([∗ map] k ↦ v ∈ m', k ↪[γ] v).
+  Proof.
+    unseal. intros ?. rewrite -big_opM_own_1 -own_op.
+    apply own_update. apply: juicy_view_alloc_big; done.
+  Qed.
+  Lemma resource_map_insert_persist_big {γ m} m' :
+    m' ##ₘ m →
+    resource_map_auth γ Tsh m ==∗
+    resource_map_auth γ Tsh (m' ∪ m) ∗ ([∗ map] k ↦ v ∈ m', k ↪[γ]□ v).
+  Proof.
+    iIntros (Hdisj) "Hauth".
+    iMod (resource_map_insert_big m' with "Hauth") as "[$ Helem]".
+    iApply big_sepM_bupd. iApply (big_sepM_impl with "Helem").
+    iIntros "!#" (k v) "_". iApply resource_map_elem_persist.
+  Qed.
+
+  Lemma resource_map_delete_big {γ m} m0 :
+    resource_map_auth γ Tsh m -∗
+    ([∗ map] k↦v ∈ m0, k ↪[γ] v) ==∗
+    resource_map_auth γ Tsh (m ∖ m0).
+  Proof.
+    iIntros "Hauth Hfrag". iMod (resource_map_elems_unseal with "Hfrag") as "Hfrag".
+    unseal. iApply (own_update_2 with "Hauth Hfrag").
+    apply: juicy_view_delete_big.
+  Qed.
+
+  Theorem resource_map_update_big {γ m} m0 m1 :
+    dom m0 = dom m1 →
+    resource_map_auth γ Tsh m -∗
+    ([∗ map] k↦v ∈ m0, k ↪[γ] v) ==∗
+    resource_map_auth γ Tsh (m1 ∪ m) ∗
+        [∗ map] k↦v ∈ m1, k ↪[γ] v.
+  Proof.
+    iIntros (?) "Hauth Hfrag". iMod (resource_map_elems_unseal with "Hfrag") as "Hfrag".
+    unseal. rewrite -big_opM_own_1 -own_op.
+    iApply (own_update_2 with "Hauth Hfrag").
+    apply: juicy_view_update_big. done.
+  Qed. *)
+
+End lemmas.
